src/ReactorModel/Components/Reactor/Properties.lean
@@ -30,7 +30,15 @@ theorem wfMutDeps {rtr : Reactor ι υ} {m : Reaction ι υ} (r : Ports.Role) (h
   have hrm := (Reaction.rawEquiv_isMut_iff hq).mp hm
   have hw := rtr.rawWF.direct.wfMutDeps mr i hr hrm
   obtain ⟨h₁, h₂⟩ := hw
-  sorry  
+  clear hw
+  apply And.intro
+  case left =>
+    clear h₂
+    sorry
+  case right =>
+    clear h₁
+    simp at h₂
+    sorry  
 
 theorem mutsBeforeNorms {rtr : Reactor ι υ} {iₙ iₘ : ι} (hn : iₙ ∈ rtr.norms.ids) (hm : iₘ ∈ rtr.muts.ids) : 
   rtr.prios.lt iₘ iₙ := by
@@ -46,7 +54,7 @@ theorem mutsBeforeNorms {rtr : Reactor ι υ} {iₙ iₘ : ι} (hn : iₙ ∈ rt
   exact h _ _ hi₁ hmr₁ hi₂ hmr₂
 
 theorem mutsLinearOrder {rtr : Reactor ι υ} {i₁ i₂ : ι} (h₁ : i₁ ∈ rtr.muts.ids) (h₂ : i₂ ∈ rtr.muts.ids) : 
-  (rtr.prios.le i₁ i₂ ∨ rtr.prios.le i₂ i₁) := by
+  rtr.prios.le i₁ i₂ ∨ rtr.prios.le i₂ i₁ := by
   have h := rtr.rawWF.direct.mutsLinearOrder i₁ i₂
   simp only [muts, Finmap.filter'_mem_ids] at h₁ h₂
   obtain ⟨hr₁, hm₁⟩ := h₁.choose_spec
@@ -58,24 +66,15 @@ theorem mutsLinearOrder {rtr : Reactor ι υ} {i₁ i₂ : ι} (h₁ : i₁ ∈ 
   have hmr₂ := (Reaction.rawEquiv_isMut_iff $ he.rel hr₂ hi₂).mp hm₂
   exact h _ _ hi₁ hi₂ hmr₁ hmr₂
 
-inductive IDPath : Reactor ι υ → ι → Type _ 
-  | rtr {σ i} : i ∈ σ.nest.ids  → IDPath σ i
-  | rcn {σ i} : i ∈ σ.rcns.ids  → IDPath σ i
-  | prt {σ i} : i ∈ σ.ports.ids → IDPath σ i
-  | stv {σ i} : i ∈ σ.state.ids → IDPath σ i
-  | nest {σ : Reactor ι υ} σ' {i} i' : (IDPath σ' i) → (σ.nest i' = some σ') → IDPath σ i
-
-namespace IDPath
-
-def cmp {σ : Reactor ι υ} {i} : IDPath σ i → Cmp
-  | rtr _ => Cmp.rtr
-  | rcn _ => Cmp.rcn
-  | prt _ => Cmp.prt
-  | stv _ => Cmp.stv
-  | nest _ _ p _ => p.cmp
+inductive Lineage : Reactor ι υ → ι → Type _ 
+  | rtr {σ i} : i ∈ σ.nest.ids  → Lineage σ i
+  | rcn {σ i} : i ∈ σ.rcns.ids  → Lineage σ i
+  | prt {σ i} : i ∈ σ.ports.ids → Lineage σ i
+  | stv {σ i} : i ∈ σ.state.ids → Lineage σ i
+  | nest {σ : Reactor ι υ} σ' {i} i' : (Lineage σ' i) → (σ.nest i' = some σ') → Lineage σ i
 
 -- Returns the reactor that matches the last ID in the ID-path (along with the ID).
-def last {σ : Reactor ι υ} {i} : IDPath σ i → (ι × Reactor ι υ)
+def Lineage.last {σ : Reactor ι υ} {i} : Lineage σ i → (ι × Reactor ι υ)
   | rtr _ => (⊤, σ)
   | rcn _ => (⊤, σ)
   | prt _ => (⊤, σ)
@@ -84,30 +83,29 @@ def last {σ : Reactor ι υ} {i} : IDPath σ i → (ι × Reactor ι υ)
   | nest σ' i' (rcn _ ) _ => (i', σ')
   | nest σ' i' (prt _ ) _ => (i', σ')
   | nest σ' i' (stv _ ) _ => (i', σ')
-  | nest _ _ p _ => last p
+  | nest _ _ l _ => last l
 
-private def toRaw {σ : Reactor ι υ} {i} : (IDPath σ i) → Raw.Reactor.IDPath σ.raw i
-  | IDPath.prt h => Raw.Reactor.IDPath.prt σ.raw i h
-  | IDPath.stv h => Raw.Reactor.IDPath.stv σ.raw i h
-  | IDPath.rcn h => Raw.Reactor.IDPath.rcn σ.raw i $ ((rcns_rawEquiv σ).eqIDs i).mp h
-  | IDPath.rtr h => Raw.Reactor.IDPath.rtr σ.raw i $ ((nest_rawEquiv σ).eqIDs i).mp h
-  | IDPath.nest _ i' p hn => Raw.Reactor.IDPath.nest σ.raw i i' (toRaw p) (nest_rawEquiv' hn)
-
-end IDPath
-
-theorem uniqueIDs {σ : Reactor ι υ} {i} (p₁ p₂ : IDPath σ i) : p₁ = p₂ := by
-  have h := σ.rawWF.direct.uniqueIDs p₁.toRaw p₂.toRaw
-  induction p₁
+-- https://leanprover.zulipchat.com/#narrow/stream/270676-lean4/topic/Unfold.20where
+theorem uniqueIDs {σ : Reactor ι υ} {i} (l₁ l₂ : Lineage σ i) : l₁ = l₂ := by
+  have h := σ.rawWF.direct.uniqueIDs (toRaw l₁) (toRaw l₂)
+  induction l₁
   case nest _ σ₂ _ _ _ _ hi =>
-    cases p₂ 
+    cases l₂ 
     case nest σ' _ _ _ =>
-      simp [IDPath.toRaw] at h
+      simp [toRaw] at h
       have hσ : σ₂ = σ' := by ext; exact h.left
       subst hσ
       simp [h.right.left]
       exact hi _ $ eq_of_heq h.right.right
     all_goals { contradiction }
-  all_goals { cases p₂ <;> simp [IDPath.toRaw] at * }
+  all_goals { cases l₂ <;> simp [toRaw] at * }
+where
+  toRaw {σ : Reactor ι υ} {i} : (Lineage σ i) → Raw.Reactor.Lineage σ.raw i
+    | Lineage.prt h => Raw.Reactor.Lineage.prt σ.raw i h
+    | Lineage.stv h => Raw.Reactor.Lineage.stv σ.raw i h
+    | Lineage.rcn h => Raw.Reactor.Lineage.rcn σ.raw i $ ((rcns_rawEquiv σ).eqIDs i).mp h
+    | Lineage.rtr h => Raw.Reactor.Lineage.rtr σ.raw i $ ((nest_rawEquiv σ).eqIDs i).mp h
+    | Lineage.nest _ i' l hn => Raw.Reactor.Lineage.nest σ.raw i i' (toRaw l) (nest_rawEquiv' hn)
 
 -- https://leanprover.zulipchat.com/#narrow/stream/270676-lean4/topic/Name.20structure.20constructor
 -- TODO: Figure out how to make a "proper" constructor for `Reactor`.
